hs/src/TLS.hs
@@ -146,9 +146,9 @@ type Handshake13 = I.Handshake13
 
 type Packet13 = I.Packet13
 
-type PublicKey = RSA.PublicKey
+type PublicKey = X.PubKey
 
-type PrivateKey = RSA.PrivateKey
+type PrivateKey = X.PrivKey
 
 type GroupPublic = I.GroupPublic
 
@@ -158,14 +158,17 @@ type Hash = T.Hash
 
 type Cipher = T.Cipher
 
+type HashAndSignatureAlgorithm = I.HashAndSignatureAlgorithm
+
 data Eff_tls =
    RecvClientHello
  | RecvFinished
  | RecvCCS
+ | RecvAppData
  | GetRandomBytes
  | SendPacket
- | GenKeys
  | GroupGetPubShared
+ | MakeCertVerify
 
 type Args_tls = Any
 
@@ -187,6 +190,10 @@ lift_tls e a e0 =
     case e0 of {
      RecvCCS -> a;
      _ -> (\_ -> Prelude.Right GHC.Base.Nothing)};
+   RecvAppData ->
+    case e0 of {
+     RecvAppData -> a;
+     _ -> (\_ -> Prelude.Right GHC.Base.Nothing)};
    GetRandomBytes ->
     case e0 of {
      GetRandomBytes -> a;
@@ -195,13 +202,13 @@ lift_tls e a e0 =
     case e0 of {
      SendPacket -> a;
      _ -> (\_ -> Prelude.Right GHC.Base.Nothing)};
-   GenKeys ->
-    case e0 of {
-     GenKeys -> a;
-     _ -> (\_ -> Prelude.Right GHC.Base.Nothing)};
    GroupGetPubShared ->
     case e0 of {
      GroupGetPubShared -> a;
+     _ -> (\_ -> Prelude.Right GHC.Base.Nothing)};
+   MakeCertVerify ->
+    case e0 of {
+     MakeCertVerify -> a;
      _ -> (\_ -> Prelude.Right GHC.Base.Nothing)}}
 
 cipherID_beq :: CipherID -> CipherID -> GHC.Base.Bool
@@ -241,10 +248,16 @@ serverHello13 = (\b -> I.ServerHello13 (I.ServerRandom {I.unServerRandom = b}))
 changeCipherSpec :: Packet13
 changeCipherSpec = I.ChangeCipherSpec13
 
+extension_SignatureAlgorithms :: (([]) ExtensionRaw) -> ([])
+                                 HashAndSignatureAlgorithm
+extension_SignatureAlgorithms = (\exts -> case Helper.extensionLookup I.extensionID_SignatureAlgorithms exts GHC.Base.>>= I.extensionDecode I.MsgTClientHello of { GHC.Base.Just (I.SignatureAlgorithms sas) -> sas })
+
+type Certificate = X.Certificate
+
 type CertificateChain = X.CertificateChain
 
-defaultCertChain :: PublicKey -> CertificateChain
-defaultCertChain = Helper.defaultCertChain
+getCertificates :: CertificateChain -> ([]) Certificate
+getCertificates = \cch -> case cch of { X.CertificateChain certs -> Prelude.map X.getCertificate certs }
 
 certificate13 :: ByteString -> CertificateChain -> (([]) (([]) ExtensionRaw)) ->
                  Handshake13
@@ -259,11 +272,11 @@ ciphersuite_default = I.ciphersuite_default
 hashWith :: Hash -> (([]) ByteString) -> ByteString
 hashWith = Helper.hashWith
 
-makeCertVerify :: PrivateKey -> ByteString -> Handshake13
-makeCertVerify = Helper.makeCertVerify
-
 encryptedExtensions13 :: (([]) ExtensionRaw) -> Handshake13
 encryptedExtensions13 = I.EncryptedExtensions13
+
+appData13 :: ByteString -> Packet13
+appData13 = I.AppData13
 
 type CryptoError = I.CryptoError
 
@@ -322,373 +335,516 @@ makeVerifyData h key transcript =
       (s2b ((:) 'f' ((:) 'i' ((:) 'n' ((:) 'i' ((:) 's' ((:) 'h' ((:) 'e' ((:) 'd'
         ([])))))))))) (s2b ([])) (hashDigestSize h)) transcript
 
-doHandshake_step :: (Prelude.Either ()
-                    (Prelude.Either ()
-                    (Prelude.Either
-                    ((,)
-                    ((,) ((,) ((,) () ((,) ClientHelloMsg ByteString)) Cipher)
-                    I.KeyShareEntry) GroupPublic)
-                    (Prelude.Either
-                    ((,)
-                    ((,) ((,) ((,) () ((,) ClientHelloMsg ByteString)) Cipher)
-                    I.KeyShareEntry) ((,) GroupPublic GroupKey))
-                    (Prelude.Either
-                    ((,)
-                    ((,)
-                    ((,) ((,) ((,) () ((,) ClientHelloMsg ByteString)) Cipher)
-                    I.KeyShareEntry) ((,) GroupPublic GroupKey)) ByteString)
-                    (Prelude.Either
-                    ((,)
-                    ((,) ((,) ((,) () ((,) ClientHelloMsg ByteString)) Cipher)
-                    ((,) GroupPublic GroupKey)) ByteString)
-                    (Prelude.Either
-                    ((,)
-                    ((,) ((,) ((,) () ((,) ClientHelloMsg ByteString)) Cipher)
-                    ((,) GroupPublic GroupKey)) ByteString)
-                    (Prelude.Either
-                    ((,)
-                    ((,)
-                    ((,) ((,) ((,) () ((,) ClientHelloMsg ByteString)) Cipher)
-                    ((,) GroupPublic GroupKey)) ByteString) ByteString)
-                    (Prelude.Either
-                    ((,)
-                    ((,)
-                    ((,)
-                    ((,) ((,) ((,) () ((,) ClientHelloMsg ByteString)) Cipher)
-                    ((,) GroupPublic GroupKey)) ByteString) ByteString)
-                    ((,) PublicKey PrivateKey))
-                    (Prelude.Either
-                    ((,)
-                    ((,)
-                    ((,)
-                    ((,)
-                    ((,) ((,) ((,) () ((,) ClientHelloMsg ByteString)) Cipher)
-                    ((,) GroupPublic GroupKey)) ByteString) ByteString)
-                    ((,) PublicKey PrivateKey)) ByteString)
+isDigitalSignaturePair :: ((,) PublicKey PrivateKey) -> GHC.Base.Bool
+isDigitalSignaturePair = I.isDigitalSignaturePair
+
+signatureCompatible13 :: PublicKey -> HashAndSignatureAlgorithm -> GHC.Base.Bool
+signatureCompatible13 = I.signatureCompatible13
+
+certPubKey :: Certificate -> PublicKey
+certPubKey = X.certPubKey
+
+decideCredInfo' :: PrivateKey -> HashAndSignatureAlgorithm -> (([]) Certificate) ->
+                   GHC.Base.Maybe ((,) PublicKey HashAndSignatureAlgorithm)
+decideCredInfo' priv hashSig certs =
+  case certs of {
+   [] -> GHC.Base.Nothing;
+   (:) cert rest ->
+    let {pub = certPubKey cert} in
+    case isDigitalSignaturePair ((,) pub priv) of {
+     GHC.Base.True ->
+      case signatureCompatible13 pub hashSig of {
+       GHC.Base.True -> GHC.Base.Just ((,) pub hashSig);
+       GHC.Base.False -> decideCredInfo' priv hashSig rest};
+     GHC.Base.False -> decideCredInfo' priv hashSig rest}}
+
+decideCredInfo :: PrivateKey -> (([]) Certificate) -> (([])
+                  HashAndSignatureAlgorithm) -> GHC.Base.Maybe
+                  ((,) PublicKey HashAndSignatureAlgorithm)
+decideCredInfo priv certs hashSigs =
+  case hashSigs of {
+   [] -> GHC.Base.Nothing;
+   (:) hashSig rest ->
+    case decideCredInfo' priv hashSig certs of {
+     GHC.Base.Just res -> GHC.Base.Just res;
+     GHC.Base.Nothing -> decideCredInfo priv certs rest}}
+
+doHandshake_step :: (Prelude.Either ((,) ((,) () CertificateChain) PrivateKey)
+                    (Prelude.Either ((,) ((,) () CertificateChain) PrivateKey)
                     (Prelude.Either
                     ((,)
                     ((,)
                     ((,)
-                    ((,)
-                    ((,)
-                    ((,) ((,) ((,) () ((,) ClientHelloMsg ByteString)) Cipher)
-                    ((,) GroupPublic GroupKey)) ByteString) ByteString)
-                    ((,) PublicKey PrivateKey)) ByteString) ByteString)
+                    ((,) ((,) ((,) () CertificateChain) PrivateKey)
+                    ((,) ClientHelloMsg ByteString)) Cipher) I.KeyShareEntry)
+                    GroupPublic)
                     (Prelude.Either
                     ((,)
                     ((,)
                     ((,)
-                    ((,)
-                    ((,)
-                    ((,)
-                    ((,) ((,) ((,) () ((,) ClientHelloMsg ByteString)) Cipher)
-                    ((,) GroupPublic GroupKey)) ByteString) ByteString)
-                    ((,) PublicKey PrivateKey)) ByteString) ByteString) ByteString)
+                    ((,) ((,) ((,) () CertificateChain) PrivateKey)
+                    ((,) ClientHelloMsg ByteString)) Cipher) I.KeyShareEntry)
+                    ((,) GroupPublic GroupKey))
                     (Prelude.Either
                     ((,)
                     ((,)
                     ((,)
                     ((,)
-                    ((,)
-                    ((,)
-                    ((,) ((,) ((,) () ((,) ClientHelloMsg ByteString)) Cipher)
-                    ((,) GroupPublic GroupKey)) ByteString) ByteString)
-                    ((,) PublicKey PrivateKey)) ByteString) ByteString) ByteString)
-                    (GHC.Base.Maybe
-                    ((,) ((,) ((,) ByteString ByteString) Handshake13) PublicKey)))))))))))))))
-                    -> Eff_tls -> Rets_tls -> Prelude.Either
-                    ((,)
-                    (Prelude.Either ()
-                    (Prelude.Either ()
-                    (Prelude.Either
-                    ((,)
-                    ((,) ((,) ((,) () ((,) ClientHelloMsg ByteString)) Cipher)
-                    I.KeyShareEntry) GroupPublic)
-                    (Prelude.Either
-                    ((,)
-                    ((,) ((,) ((,) () ((,) ClientHelloMsg ByteString)) Cipher)
-                    I.KeyShareEntry) ((,) GroupPublic GroupKey))
-                    (Prelude.Either
-                    ((,)
-                    ((,)
-                    ((,) ((,) ((,) () ((,) ClientHelloMsg ByteString)) Cipher)
-                    I.KeyShareEntry) ((,) GroupPublic GroupKey)) ByteString)
-                    (Prelude.Either
-                    ((,)
-                    ((,) ((,) ((,) () ((,) ClientHelloMsg ByteString)) Cipher)
-                    ((,) GroupPublic GroupKey)) ByteString)
-                    (Prelude.Either
-                    ((,)
-                    ((,) ((,) ((,) () ((,) ClientHelloMsg ByteString)) Cipher)
+                    ((,) ((,) ((,) () CertificateChain) PrivateKey)
+                    ((,) ClientHelloMsg ByteString)) Cipher) I.KeyShareEntry)
                     ((,) GroupPublic GroupKey)) ByteString)
                     (Prelude.Either
                     ((,)
                     ((,)
-                    ((,) ((,) ((,) () ((,) ClientHelloMsg ByteString)) Cipher)
-                    ((,) GroupPublic GroupKey)) ByteString) ByteString)
+                    ((,)
+                    ((,) ((,) ((,) () CertificateChain) PrivateKey)
+                    ((,) ClientHelloMsg ByteString)) Cipher)
+                    ((,) GroupPublic GroupKey)) ByteString)
                     (Prelude.Either
                     ((,)
                     ((,)
                     ((,)
-                    ((,) ((,) ((,) () ((,) ClientHelloMsg ByteString)) Cipher)
-                    ((,) GroupPublic GroupKey)) ByteString) ByteString)
-                    ((,) PublicKey PrivateKey))
-                    (Prelude.Either
-                    ((,)
-                    ((,)
-                    ((,)
-                    ((,)
-                    ((,) ((,) ((,) () ((,) ClientHelloMsg ByteString)) Cipher)
-                    ((,) GroupPublic GroupKey)) ByteString) ByteString)
-                    ((,) PublicKey PrivateKey)) ByteString)
+                    ((,) ((,) ((,) () CertificateChain) PrivateKey)
+                    ((,) ClientHelloMsg ByteString)) Cipher)
+                    ((,) GroupPublic GroupKey)) ByteString)
                     (Prelude.Either
                     ((,)
                     ((,)
                     ((,)
                     ((,)
                     ((,)
-                    ((,) ((,) ((,) () ((,) ClientHelloMsg ByteString)) Cipher)
+                    ((,) ((,) ((,) () CertificateChain) PrivateKey)
+                    ((,) ClientHelloMsg ByteString)) Cipher)
                     ((,) GroupPublic GroupKey)) ByteString) ByteString)
-                    ((,) PublicKey PrivateKey)) ByteString) ByteString)
+                    ((,) PublicKey HashAndSignatureAlgorithm))
                     (Prelude.Either
                     ((,)
                     ((,)
                     ((,)
                     ((,)
                     ((,)
+                    ((,) ((,) ((,) () PrivateKey) ((,) ClientHelloMsg ByteString))
+                    Cipher) ((,) GroupPublic GroupKey)) ByteString) ByteString)
+                    ((,) PublicKey HashAndSignatureAlgorithm)) ByteString)
+                    (Prelude.Either
+                    ((,)
+                    ((,)
+                    ((,)
                     ((,)
                     ((,) ((,) ((,) () ((,) ClientHelloMsg ByteString)) Cipher)
-                    ((,) GroupPublic GroupKey)) ByteString) ByteString)
-                    ((,) PublicKey PrivateKey)) ByteString) ByteString) ByteString)
+                    ((,) GroupPublic GroupKey)) ByteString) ByteString) ByteString)
+                    Handshake13)
+                    (Prelude.Either
+                    ((,)
+                    ((,)
+                    ((,)
+                    ((,)
+                    ((,) ((,) ((,) () ((,) ClientHelloMsg ByteString)) Cipher)
+                    ((,) GroupPublic GroupKey)) ByteString) ByteString) ByteString)
+                    ByteString)
                     (Prelude.Either
                     ((,)
                     ((,)
                     ((,)
                     ((,)
                     ((,)
+                    ((,) ((,) ((,) () ((,) ClientHelloMsg ByteString)) Cipher)
+                    ((,) GroupPublic GroupKey)) ByteString) ByteString) ByteString)
+                    ByteString) ByteString)
+                    (Prelude.Either
+                    ((,)
+                    ((,)
+                    ((,)
+                    ((,)
                     ((,)
                     ((,) ((,) ((,) () ((,) ClientHelloMsg ByteString)) Cipher)
+                    ((,) GroupPublic GroupKey)) ByteString) ByteString) ByteString)
+                    ByteString) ByteString)
+                    (Prelude.Either
+                    ((,)
+                    ((,)
+                    ((,)
+                    ((,)
+                    ((,)
+                    ((,) ((,) ((,) () ((,) ClientHelloMsg ByteString)) Cipher)
+                    ((,) GroupPublic GroupKey)) ByteString) ByteString) ByteString)
+                    ByteString) ByteString) (GHC.Base.Maybe ()))))))))))))))) ->
+                    Eff_tls -> Rets_tls -> Prelude.Either
+                    ((,)
+                    (Prelude.Either ((,) ((,) () CertificateChain) PrivateKey)
+                    (Prelude.Either ((,) ((,) () CertificateChain) PrivateKey)
+                    (Prelude.Either
+                    ((,)
+                    ((,)
+                    ((,)
+                    ((,) ((,) ((,) () CertificateChain) PrivateKey)
+                    ((,) ClientHelloMsg ByteString)) Cipher) I.KeyShareEntry)
+                    GroupPublic)
+                    (Prelude.Either
+                    ((,)
+                    ((,)
+                    ((,)
+                    ((,) ((,) ((,) () CertificateChain) PrivateKey)
+                    ((,) ClientHelloMsg ByteString)) Cipher) I.KeyShareEntry)
+                    ((,) GroupPublic GroupKey))
+                    (Prelude.Either
+                    ((,)
+                    ((,)
+                    ((,)
+                    ((,)
+                    ((,) ((,) ((,) () CertificateChain) PrivateKey)
+                    ((,) ClientHelloMsg ByteString)) Cipher) I.KeyShareEntry)
+                    ((,) GroupPublic GroupKey)) ByteString)
+                    (Prelude.Either
+                    ((,)
+                    ((,)
+                    ((,)
+                    ((,) ((,) ((,) () CertificateChain) PrivateKey)
+                    ((,) ClientHelloMsg ByteString)) Cipher)
+                    ((,) GroupPublic GroupKey)) ByteString)
+                    (Prelude.Either
+                    ((,)
+                    ((,)
+                    ((,)
+                    ((,) ((,) ((,) () CertificateChain) PrivateKey)
+                    ((,) ClientHelloMsg ByteString)) Cipher)
+                    ((,) GroupPublic GroupKey)) ByteString)
+                    (Prelude.Either
+                    ((,)
+                    ((,)
+                    ((,)
+                    ((,)
+                    ((,)
+                    ((,) ((,) ((,) () CertificateChain) PrivateKey)
+                    ((,) ClientHelloMsg ByteString)) Cipher)
                     ((,) GroupPublic GroupKey)) ByteString) ByteString)
-                    ((,) PublicKey PrivateKey)) ByteString) ByteString) ByteString)
-                    (GHC.Base.Maybe
-                    ((,) ((,) ((,) ByteString ByteString) Handshake13) PublicKey)))))))))))))))
-                    (GHC.Base.Maybe (SigT Eff_tls Args_tls)))
-                    (GHC.Base.Maybe
-                    ((,) ((,) ((,) ByteString ByteString) Handshake13) PublicKey))
+                    ((,) PublicKey HashAndSignatureAlgorithm))
+                    (Prelude.Either
+                    ((,)
+                    ((,)
+                    ((,)
+                    ((,)
+                    ((,)
+                    ((,) ((,) ((,) () PrivateKey) ((,) ClientHelloMsg ByteString))
+                    Cipher) ((,) GroupPublic GroupKey)) ByteString) ByteString)
+                    ((,) PublicKey HashAndSignatureAlgorithm)) ByteString)
+                    (Prelude.Either
+                    ((,)
+                    ((,)
+                    ((,)
+                    ((,)
+                    ((,) ((,) ((,) () ((,) ClientHelloMsg ByteString)) Cipher)
+                    ((,) GroupPublic GroupKey)) ByteString) ByteString) ByteString)
+                    Handshake13)
+                    (Prelude.Either
+                    ((,)
+                    ((,)
+                    ((,)
+                    ((,)
+                    ((,) ((,) ((,) () ((,) ClientHelloMsg ByteString)) Cipher)
+                    ((,) GroupPublic GroupKey)) ByteString) ByteString) ByteString)
+                    ByteString)
+                    (Prelude.Either
+                    ((,)
+                    ((,)
+                    ((,)
+                    ((,)
+                    ((,)
+                    ((,) ((,) ((,) () ((,) ClientHelloMsg ByteString)) Cipher)
+                    ((,) GroupPublic GroupKey)) ByteString) ByteString) ByteString)
+                    ByteString) ByteString)
+                    (Prelude.Either
+                    ((,)
+                    ((,)
+                    ((,)
+                    ((,)
+                    ((,)
+                    ((,) ((,) ((,) () ((,) ClientHelloMsg ByteString)) Cipher)
+                    ((,) GroupPublic GroupKey)) ByteString) ByteString) ByteString)
+                    ByteString) ByteString)
+                    (Prelude.Either
+                    ((,)
+                    ((,)
+                    ((,)
+                    ((,)
+                    ((,)
+                    ((,) ((,) ((,) () ((,) ClientHelloMsg ByteString)) Cipher)
+                    ((,) GroupPublic GroupKey)) ByteString) ByteString) ByteString)
+                    ByteString) ByteString) (GHC.Base.Maybe ())))))))))))))))
+                    (GHC.Base.Maybe (SigT Eff_tls Args_tls))) (GHC.Base.Maybe ())
 doHandshake_step =
-  sum_merge (\_ _ _ -> Prelude.Left ((,) (Prelude.Right (Prelude.Left ()))
-    (GHC.Base.Just (ExistT RecvClientHello (unsafeCoerce ())))))
-    (sum_merge (\_ ->
-      lift_tls RecvClientHello (\r -> Prelude.Left ((,)
-        (case chooseCipher (chCiphers (fst (unsafeCoerce r))) ciphersuite_default of {
-          GHC.Base.Just a ->
-           case extension_KeyShare (chExtension (fst (unsafeCoerce r))) of {
-            GHC.Base.Just a0 ->
-             case findKeyShare a0 serverGroups of {
-              GHC.Base.Just a1 ->
-               case decodeGroupPublic (ksGroup a1) (ksData a1) of {
-                Prelude.Left _ -> Prelude.Right (Prelude.Right (Prelude.Right
+  sum_merge
+    (prod_curry
+      (prod_curry (\_ c p _ _ -> Prelude.Left ((,) (Prelude.Right (Prelude.Left ((,)
+        ((,) () c) p))) (GHC.Base.Just (ExistT RecvClientHello
+        (unsafeCoerce ())))))))
+    (sum_merge
+      (prod_curry
+        (prod_curry (\_ c p ->
+          lift_tls RecvClientHello (\r -> Prelude.Left ((,)
+            (case chooseCipher (chCiphers (fst (unsafeCoerce r)))
+                    ciphersuite_default of {
+              GHC.Base.Just a ->
+               case extension_KeyShare (chExtension (fst (unsafeCoerce r))) of {
+                GHC.Base.Just a0 ->
+                 case findKeyShare a0 serverGroups of {
+                  GHC.Base.Just a1 ->
+                   case decodeGroupPublic (ksGroup a1) (ksData a1) of {
+                    Prelude.Left _ -> Prelude.Right (Prelude.Right (Prelude.Right
+                     (Prelude.Right (Prelude.Right (Prelude.Right (Prelude.Right
+                     (Prelude.Right (Prelude.Right (Prelude.Right (Prelude.Right
+                     (Prelude.Right (Prelude.Right (Prelude.Right
+                     GHC.Base.Nothing)))))))))))));
+                    Prelude.Right b -> Prelude.Right (Prelude.Right (Prelude.Left
+                     ((,) ((,) ((,) ((,) ((,) ((,) () c) p) (unsafeCoerce r)) a) a1)
+                     b)))};
+                  GHC.Base.Nothing -> Prelude.Right (Prelude.Right (Prelude.Right
+                   (Prelude.Right (Prelude.Right (Prelude.Right (Prelude.Right
+                   (Prelude.Right (Prelude.Right (Prelude.Right (Prelude.Right
+                   (Prelude.Right (Prelude.Right (Prelude.Right
+                   GHC.Base.Nothing)))))))))))))};
+                GHC.Base.Nothing -> Prelude.Right (Prelude.Right (Prelude.Right
                  (Prelude.Right (Prelude.Right (Prelude.Right (Prelude.Right
                  (Prelude.Right (Prelude.Right (Prelude.Right (Prelude.Right
-                 (Prelude.Right (Prelude.Right GHC.Base.Nothing))))))))))));
-                Prelude.Right b -> Prelude.Right (Prelude.Right (Prelude.Left ((,)
-                 ((,) ((,) ((,) () (unsafeCoerce r)) a) a1) b)))};
+                 (Prelude.Right (Prelude.Right (Prelude.Right
+                 GHC.Base.Nothing)))))))))))))};
               GHC.Base.Nothing -> Prelude.Right (Prelude.Right (Prelude.Right
                (Prelude.Right (Prelude.Right (Prelude.Right (Prelude.Right
                (Prelude.Right (Prelude.Right (Prelude.Right (Prelude.Right
-               (Prelude.Right (Prelude.Right GHC.Base.Nothing))))))))))))};
-            GHC.Base.Nothing -> Prelude.Right (Prelude.Right (Prelude.Right
-             (Prelude.Right (Prelude.Right (Prelude.Right (Prelude.Right
-             (Prelude.Right (Prelude.Right (Prelude.Right (Prelude.Right
-             (Prelude.Right (Prelude.Right GHC.Base.Nothing))))))))))))};
-          GHC.Base.Nothing -> Prelude.Right (Prelude.Right (Prelude.Right
-           (Prelude.Right (Prelude.Right (Prelude.Right (Prelude.Right
-           (Prelude.Right (Prelude.Right (Prelude.Right (Prelude.Right
-           (Prelude.Right (Prelude.Right GHC.Base.Nothing))))))))))))})
-        (case chooseCipher (chCiphers (fst (unsafeCoerce r))) ciphersuite_default of {
-          GHC.Base.Just _ ->
-           case extension_KeyShare (chExtension (fst (unsafeCoerce r))) of {
-            GHC.Base.Just a ->
-             case findKeyShare a serverGroups of {
-              GHC.Base.Just a0 ->
-               case decodeGroupPublic (ksGroup a0) (ksData a0) of {
-                Prelude.Left _ -> GHC.Base.Nothing;
-                Prelude.Right b -> GHC.Base.Just (ExistT GroupGetPubShared
-                 (unsafeCoerce b))};
-              GHC.Base.Nothing -> GHC.Base.Nothing};
-            GHC.Base.Nothing -> GHC.Base.Nothing};
-          GHC.Base.Nothing -> GHC.Base.Nothing}))))
+               (Prelude.Right (Prelude.Right (Prelude.Right
+               GHC.Base.Nothing)))))))))))))})
+            (case chooseCipher (chCiphers (fst (unsafeCoerce r)))
+                    ciphersuite_default of {
+              GHC.Base.Just _ ->
+               case extension_KeyShare (chExtension (fst (unsafeCoerce r))) of {
+                GHC.Base.Just a ->
+                 case findKeyShare a serverGroups of {
+                  GHC.Base.Just a0 ->
+                   case decodeGroupPublic (ksGroup a0) (ksData a0) of {
+                    Prelude.Left _ -> GHC.Base.Nothing;
+                    Prelude.Right b -> GHC.Base.Just (ExistT GroupGetPubShared
+                     (unsafeCoerce b))};
+                  GHC.Base.Nothing -> GHC.Base.Nothing};
+                GHC.Base.Nothing -> GHC.Base.Nothing};
+              GHC.Base.Nothing -> GHC.Base.Nothing}))))))
       (sum_merge
         (prod_curry
           (prod_curry
             (prod_curry
-              (prod_curry (\_ r c k _ ->
-                lift_tls GroupGetPubShared (\r0 -> Prelude.Left ((,)
-                  (case unsafeCoerce r0 of {
-                    GHC.Base.Just a -> Prelude.Right (Prelude.Right (Prelude.Right
-                     (Prelude.Left ((,) ((,) ((,) ((,) () r) c) k) a))));
-                    GHC.Base.Nothing -> Prelude.Right (Prelude.Right (Prelude.Right
-                     (Prelude.Right (Prelude.Right (Prelude.Right (Prelude.Right
-                     (Prelude.Right (Prelude.Right (Prelude.Right (Prelude.Right
-                     (Prelude.Right (Prelude.Right GHC.Base.Nothing))))))))))))})
-                  (case unsafeCoerce r0 of {
-                    GHC.Base.Just _ -> GHC.Base.Just (ExistT GetRandomBytes
-                     (unsafeCoerce ((Prelude.+) 1 ((Prelude.+) 1 ((Prelude.+) 1
-                       ((Prelude.+) 1 ((Prelude.+) 1 ((Prelude.+) 1 ((Prelude.+) 1
-                       ((Prelude.+) 1 ((Prelude.+) 1 ((Prelude.+) 1 ((Prelude.+) 1
-                       ((Prelude.+) 1 ((Prelude.+) 1 ((Prelude.+) 1 ((Prelude.+) 1
-                       ((Prelude.+) 1 ((Prelude.+) 1 ((Prelude.+) 1 ((Prelude.+) 1
-                       ((Prelude.+) 1 ((Prelude.+) 1 ((Prelude.+) 1 ((Prelude.+) 1
-                       ((Prelude.+) 1 ((Prelude.+) 1 ((Prelude.+) 1 ((Prelude.+) 1
-                       ((Prelude.+) 1 ((Prelude.+) 1 ((Prelude.+) 1 ((Prelude.+) 1
-                       ((Prelude.+) 1 0))))))))))))))))))))))))))))))))));
-                    GHC.Base.Nothing -> GHC.Base.Nothing}))))))))
+              (prod_curry
+                (prod_curry
+                  (prod_curry (\_ c p r c0 k _ ->
+                    lift_tls GroupGetPubShared (\r0 -> Prelude.Left ((,)
+                      (case unsafeCoerce r0 of {
+                        GHC.Base.Just a -> Prelude.Right (Prelude.Right
+                         (Prelude.Right (Prelude.Left ((,) ((,) ((,) ((,) ((,) ((,)
+                         () c) p) r) c0) k) a))));
+                        GHC.Base.Nothing -> Prelude.Right (Prelude.Right
+                         (Prelude.Right (Prelude.Right (Prelude.Right (Prelude.Right
+                         (Prelude.Right (Prelude.Right (Prelude.Right (Prelude.Right
+                         (Prelude.Right (Prelude.Right (Prelude.Right (Prelude.Right
+                         GHC.Base.Nothing)))))))))))))})
+                      (case unsafeCoerce r0 of {
+                        GHC.Base.Just _ -> GHC.Base.Just (ExistT GetRandomBytes
+                         (unsafeCoerce ((Prelude.+) 1 ((Prelude.+) 1 ((Prelude.+) 1
+                           ((Prelude.+) 1 ((Prelude.+) 1 ((Prelude.+) 1
+                           ((Prelude.+) 1 ((Prelude.+) 1 ((Prelude.+) 1
+                           ((Prelude.+) 1 ((Prelude.+) 1 ((Prelude.+) 1
+                           ((Prelude.+) 1 ((Prelude.+) 1 ((Prelude.+) 1
+                           ((Prelude.+) 1 ((Prelude.+) 1 ((Prelude.+) 1
+                           ((Prelude.+) 1 ((Prelude.+) 1 ((Prelude.+) 1
+                           ((Prelude.+) 1 ((Prelude.+) 1 ((Prelude.+) 1
+                           ((Prelude.+) 1 ((Prelude.+) 1 ((Prelude.+) 1
+                           ((Prelude.+) 1 ((Prelude.+) 1 ((Prelude.+) 1
+                           ((Prelude.+) 1 ((Prelude.+) 1
+                           0))))))))))))))))))))))))))))))))));
+                        GHC.Base.Nothing -> GHC.Base.Nothing}))))))))))
         (sum_merge
           (prod_curry
             (prod_curry
               (prod_curry
-                (prod_curry (\_ r c k p ->
-                  lift_tls GetRandomBytes (\r0 -> Prelude.Left ((,) (Prelude.Right
-                    (Prelude.Right (Prelude.Right (Prelude.Right (Prelude.Left ((,)
-                    ((,) ((,) ((,) ((,) () r) c) k) p) (unsafeCoerce r0)))))))
-                    (GHC.Base.Just (ExistT SendPacket
-                    (unsafeCoerce ((,)
-                      (handshake13 ((:)
-                        (serverHello13 (unsafeCoerce r0) (chSession (fst r))
-                          (cipherID c) ((:)
-                          (extensionRaw_KeyShare
-                            (extensionEncode_KeyShare (I.KeyShareEntry (ksGroup k)
-                              (encodeGroupPublic (fst p))))) ((:)
-                          (extensionRaw_SupportedVersions
-                            (extensionEncode_SupportedVersions tLS13)) []))) []))
-                      GHC.Base.Nothing)))))))))))
+                (prod_curry
+                  (prod_curry
+                    (prod_curry (\_ c p r c0 k p0 ->
+                      lift_tls GetRandomBytes (\r0 -> Prelude.Left ((,)
+                        (Prelude.Right (Prelude.Right (Prelude.Right (Prelude.Right
+                        (Prelude.Left ((,) ((,) ((,) ((,) ((,) ((,) ((,) () c) p) r)
+                        c0) k) p0) (unsafeCoerce r0))))))) (GHC.Base.Just (ExistT
+                        SendPacket
+                        (unsafeCoerce ((,)
+                          (handshake13 ((:)
+                            (serverHello13 (unsafeCoerce r0) (chSession (fst r))
+                              (cipherID c0) ((:)
+                              (extensionRaw_KeyShare
+                                (extensionEncode_KeyShare (I.KeyShareEntry
+                                  (ksGroup k) (encodeGroupPublic (fst p0))))) ((:)
+                              (extensionRaw_SupportedVersions
+                                (extensionEncode_SupportedVersions tLS13)) [])))
+                            [])) GHC.Base.Nothing)))))))))))))
           (sum_merge
             (prod_curry
               (prod_curry
                 (prod_curry
                   (prod_curry
-                    (prod_curry (\_ r c _ p _ ->
-                      lift_tls SendPacket (\r0 -> Prelude.Left ((,) (Prelude.Right
-                        (Prelude.Right (Prelude.Right (Prelude.Right (Prelude.Right
-                        (Prelude.Left ((,) ((,) ((,) ((,) () r) c) p)
-                        (unsafeCoerce r0)))))))) (GHC.Base.Just (ExistT SendPacket
-                        (unsafeCoerce ((,) changeCipherSpec GHC.Base.Nothing))))))))))))
+                    (prod_curry
+                      (prod_curry
+                        (prod_curry (\_ c p r c0 _ p0 _ ->
+                          lift_tls SendPacket (\r0 -> Prelude.Left ((,)
+                            (Prelude.Right (Prelude.Right (Prelude.Right
+                            (Prelude.Right (Prelude.Right (Prelude.Left ((,) ((,)
+                            ((,) ((,) ((,) ((,) () c) p) r) c0) p0)
+                            (unsafeCoerce r0)))))))) (GHC.Base.Just (ExistT
+                            SendPacket
+                            (unsafeCoerce ((,) changeCipherSpec GHC.Base.Nothing))))))))))))))
             (sum_merge
               (prod_curry
                 (prod_curry
                   (prod_curry
-                    (prod_curry (\_ r c p r0 ->
-                      lift_tls SendPacket (\_ -> Prelude.Left ((,) (Prelude.Right
-                        (Prelude.Right (Prelude.Right (Prelude.Right (Prelude.Right
-                        (Prelude.Right (Prelude.Left ((,) ((,) ((,) ((,) () r) c) p)
-                        r0)))))))) (GHC.Base.Just (ExistT SendPacket
-                        (unsafeCoerce ((,)
-                          (handshake13 ((:) (encryptedExtensions13 []) []))
-                          (GHC.Base.Just ((,) ((,) (cipherHash c) c)
-                          (hkdfExpandLabel (cipherHash c)
-                            (hkdfExtract (cipherHash c)
-                              (hkdfExpandLabel (cipherHash c)
-                                (hkdfExtract (cipherHash c)
-                                  (b_replicate (hashDigestSize (cipherHash c)) w0)
-                                  (b_replicate (hashDigestSize (cipherHash c)) w0))
-                                (s2b ((:) 'd' ((:) 'e' ((:) 'r' ((:) 'i' ((:) 'v'
-                                  ((:) 'e' ((:) 'd' ([])))))))))
-                                (hashWith (cipherHash c) ((:) (s2b ([])) []))
-                                (hashDigestSize (cipherHash c)))
-                              (ba_convert (snd p)))
-                            (s2b ((:) 's' ((:) ' ' ((:) 'h' ((:) 's' ((:) ' ' ((:)
-                              't' ((:) 'r' ((:) 'a' ((:) 'f' ((:) 'f' ((:) 'i' ((:)
-                              'c' ([]))))))))))))))
-                            (hashWith (cipherHash c) ((:) (snd r) ((:) r0 [])))
-                            (hashDigestSize (cipherHash c))))))))))))))))
+                    (prod_curry
+                      (prod_curry
+                        (prod_curry (\_ c p r c0 p0 r0 ->
+                          lift_tls SendPacket (\_ -> Prelude.Left ((,)
+                            (Prelude.Right (Prelude.Right (Prelude.Right
+                            (Prelude.Right (Prelude.Right (Prelude.Right
+                            (Prelude.Left ((,) ((,) ((,) ((,) ((,) ((,) () c) p) r)
+                            c0) p0) r0)))))))) (GHC.Base.Just (ExistT SendPacket
+                            (unsafeCoerce ((,)
+                              (handshake13 ((:) (encryptedExtensions13 []) []))
+                              (GHC.Base.Just ((,) ((,) ((,) (cipherHash c0) c0)
+                              (hkdfExpandLabel (cipherHash c0)
+                                (hkdfExtract (cipherHash c0)
+                                  (hkdfExpandLabel (cipherHash c0)
+                                    (hkdfExtract (cipherHash c0)
+                                      (b_replicate (hashDigestSize (cipherHash c0))
+                                        w0)
+                                      (b_replicate (hashDigestSize (cipherHash c0))
+                                        w0))
+                                    (s2b ((:) 'd' ((:) 'e' ((:) 'r' ((:) 'i' ((:)
+                                      'v' ((:) 'e' ((:) 'd' ([])))))))))
+                                    (hashWith (cipherHash c0) ((:) (s2b ([])) []))
+                                    (hashDigestSize (cipherHash c0)))
+                                  (ba_convert (snd p0)))
+                                (s2b ((:) 's' ((:) ' ' ((:) 'h' ((:) 's' ((:) ' '
+                                  ((:) 't' ((:) 'r' ((:) 'a' ((:) 'f' ((:) 'f' ((:)
+                                  'i' ((:) 'c' ([]))))))))))))))
+                                (hashWith (cipherHash c0) ((:) (snd r) ((:) r0 [])))
+                                (hashDigestSize (cipherHash c0)))) 0)))))))))))))))
               (sum_merge
                 (prod_curry
                   (prod_curry
                     (prod_curry
-                      (prod_curry (\_ r c p r0 ->
-                        lift_tls SendPacket (\r1 -> Prelude.Left ((,) (Prelude.Right
-                          (Prelude.Right (Prelude.Right (Prelude.Right
-                          (Prelude.Right (Prelude.Right (Prelude.Right (Prelude.Left
-                          ((,) ((,) ((,) ((,) ((,) () r) c) p) r0)
-                          (unsafeCoerce r1)))))))))) (GHC.Base.Just (ExistT GenKeys
-                          (unsafeCoerce ()))))))))))
+                      (prod_curry
+                        (prod_curry
+                          (prod_curry (\_ c p r c0 p0 r0 ->
+                            lift_tls SendPacket (\r1 -> Prelude.Left ((,)
+                              (case decideCredInfo p (getCertificates c)
+                                      (extension_SignatureAlgorithms
+                                        (chExtension (fst r))) of {
+                                GHC.Base.Just a -> Prelude.Right (Prelude.Right
+                                 (Prelude.Right (Prelude.Right (Prelude.Right
+                                 (Prelude.Right (Prelude.Right (Prelude.Left ((,)
+                                 ((,) ((,) ((,) ((,) ((,) ((,) ((,) () c) p) r) c0)
+                                 p0) r0) (unsafeCoerce r1)) a))))))));
+                                GHC.Base.Nothing -> Prelude.Right (Prelude.Right
+                                 (Prelude.Right (Prelude.Right (Prelude.Right
+                                 (Prelude.Right (Prelude.Right (Prelude.Right
+                                 (Prelude.Right (Prelude.Right (Prelude.Right
+                                 (Prelude.Right (Prelude.Right (Prelude.Right
+                                 GHC.Base.Nothing)))))))))))))})
+                              (case decideCredInfo p (getCertificates c)
+                                      (extension_SignatureAlgorithms
+                                        (chExtension (fst r))) of {
+                                GHC.Base.Just _ -> GHC.Base.Just (ExistT SendPacket
+                                 (unsafeCoerce ((,)
+                                   (handshake13 ((:)
+                                     (certificate13 empty c ((:) [] [])) []))
+                                   (GHC.Base.Just ((,) ((,) ((,) (cipherHash c0) c0)
+                                   (hkdfExpandLabel (cipherHash c0)
+                                     (hkdfExtract (cipherHash c0)
+                                       (hkdfExpandLabel (cipherHash c0)
+                                         (hkdfExtract (cipherHash c0)
+                                           (b_replicate
+                                             (hashDigestSize (cipherHash c0)) w0)
+                                           (b_replicate
+                                             (hashDigestSize (cipherHash c0)) w0))
+                                         (s2b ((:) 'd' ((:) 'e' ((:) 'r' ((:) 'i'
+                                           ((:) 'v' ((:) 'e' ((:) 'd' ([])))))))))
+                                         (hashWith (cipherHash c0) ((:) (s2b ([]))
+                                           [])) (hashDigestSize (cipherHash c0)))
+                                       (ba_convert (snd p0)))
+                                     (s2b ((:) 's' ((:) ' ' ((:) 'h' ((:) 's' ((:)
+                                       ' ' ((:) 't' ((:) 'r' ((:) 'a' ((:) 'f' ((:)
+                                       'f' ((:) 'i' ((:) 'c' ([]))))))))))))))
+                                     (hashWith (cipherHash c0) ((:) (snd r) ((:) r0
+                                       []))) (hashDigestSize (cipherHash c0))))
+                                   ((Prelude.+) 1 0))))));
+                                GHC.Base.Nothing -> GHC.Base.Nothing}))))))))))
                 (sum_merge
                   (prod_curry
                     (prod_curry
                       (prod_curry
                         (prod_curry
-                          (prod_curry (\_ r c p r0 r1 ->
-                            lift_tls GenKeys (\r2 -> Prelude.Left ((,)
-                              (Prelude.Right (Prelude.Right (Prelude.Right
-                              (Prelude.Right (Prelude.Right (Prelude.Right
-                              (Prelude.Right (Prelude.Right (Prelude.Left ((,) ((,)
-                              ((,) ((,) ((,) ((,) () r) c) p) r0) r1)
-                              (unsafeCoerce r2))))))))))) (GHC.Base.Just (ExistT
-                              SendPacket
-                              (unsafeCoerce ((,)
-                                (handshake13 ((:)
-                                  (certificate13 empty
-                                    (defaultCertChain (fst (unsafeCoerce r2))) ((:)
-                                    [] [])) [])) (GHC.Base.Just ((,) ((,)
-                                (cipherHash c) c)
-                                (hkdfExpandLabel (cipherHash c)
-                                  (hkdfExtract (cipherHash c)
-                                    (hkdfExpandLabel (cipherHash c)
-                                      (hkdfExtract (cipherHash c)
-                                        (b_replicate (hashDigestSize (cipherHash c))
-                                          w0)
-                                        (b_replicate (hashDigestSize (cipherHash c))
-                                          w0))
-                                      (s2b ((:) 'd' ((:) 'e' ((:) 'r' ((:) 'i' ((:)
-                                        'v' ((:) 'e' ((:) 'd' ([])))))))))
-                                      (hashWith (cipherHash c) ((:) (s2b ([])) []))
-                                      (hashDigestSize (cipherHash c)))
-                                    (ba_convert (snd p)))
-                                  (s2b ((:) 's' ((:) ' ' ((:) 'h' ((:) 's' ((:) ' '
-                                    ((:) 't' ((:) 'r' ((:) 'a' ((:) 'f' ((:) 'f'
-                                    ((:) 'i' ((:) 'c' ([]))))))))))))))
-                                  (hashWith (cipherHash c) ((:) (snd r) ((:) r0
-                                    []))) (hashDigestSize (cipherHash c)))))))))))))))))
+                          (prod_curry
+                            (prod_curry
+                              (prod_curry
+                                (prod_curry (\_ _ p r c p0 r0 r1 p1 ->
+                                  lift_tls SendPacket (\r2 -> Prelude.Left ((,)
+                                    (Prelude.Right (Prelude.Right (Prelude.Right
+                                    (Prelude.Right (Prelude.Right (Prelude.Right
+                                    (Prelude.Right (Prelude.Right (Prelude.Left ((,)
+                                    ((,) ((,) ((,) ((,) ((,) ((,) ((,) () p) r) c)
+                                    p0) r0) r1) p1) (unsafeCoerce r2)))))))))))
+                                    (GHC.Base.Just (ExistT MakeCertVerify
+                                    (unsafeCoerce ((,) ((,) ((,) (fst p1) p)
+                                      (snd p1))
+                                      (hashWith (cipherHash c) ((:) (snd r) ((:) r0
+                                        ((:) r1 ((:) (unsafeCoerce r2) []))))))))))))))))))))
                   (sum_merge
                     (prod_curry
                       (prod_curry
                         (prod_curry
                           (prod_curry
                             (prod_curry
-                              (prod_curry (\_ r c p r0 r1 r2 ->
-                                lift_tls SendPacket (\r3 -> Prelude.Left ((,)
-                                  (Prelude.Right (Prelude.Right (Prelude.Right
-                                  (Prelude.Right (Prelude.Right (Prelude.Right
-                                  (Prelude.Right (Prelude.Right (Prelude.Right
-                                  (Prelude.Left ((,) ((,) ((,) ((,) ((,) ((,) ((,)
-                                  () r) c) p) r0) r1) r2)
-                                  (unsafeCoerce r3)))))))))))) (GHC.Base.Just
-                                  (ExistT SendPacket
-                                  (unsafeCoerce ((,)
-                                    (handshake13 ((:)
-                                      (makeCertVerify (snd r2)
-                                        (hashWith (cipherHash c) ((:) (snd r) ((:)
-                                          r0 ((:) r1 ((:) (unsafeCoerce r3) []))))))
-                                      [])) (GHC.Base.Just ((,) ((,) (cipherHash c)
-                                    c)
-                                    (hkdfExpandLabel (cipherHash c)
-                                      (hkdfExtract (cipherHash c)
+                              (prod_curry
+                                (prod_curry
+                                  (prod_curry (\_ _ r c p r0 r1 _ r2 ->
+                                    lift_tls MakeCertVerify (\r3 -> Prelude.Left
+                                      ((,) (Prelude.Right (Prelude.Right
+                                      (Prelude.Right (Prelude.Right (Prelude.Right
+                                      (Prelude.Right (Prelude.Right (Prelude.Right
+                                      (Prelude.Right (Prelude.Left ((,) ((,) ((,)
+                                      ((,) ((,) ((,) ((,) () r) c) p) r0) r1) r2)
+                                      (unsafeCoerce r3)))))))))))) (GHC.Base.Just
+                                      (ExistT SendPacket
+                                      (unsafeCoerce ((,)
+                                        (handshake13 ((:) (unsafeCoerce r3) []))
+                                        (GHC.Base.Just ((,) ((,) ((,) (cipherHash c)
+                                        c)
                                         (hkdfExpandLabel (cipherHash c)
                                           (hkdfExtract (cipherHash c)
-                                            (b_replicate
-                                              (hashDigestSize (cipherHash c)) w0)
-                                            (b_replicate
-                                              (hashDigestSize (cipherHash c)) w0))
-                                          (s2b ((:) 'd' ((:) 'e' ((:) 'r' ((:) 'i'
-                                            ((:) 'v' ((:) 'e' ((:) 'd' ([])))))))))
-                                          (hashWith (cipherHash c) ((:) (s2b ([]))
-                                            [])) (hashDigestSize (cipherHash c)))
-                                        (ba_convert (snd p)))
-                                      (s2b ((:) 's' ((:) ' ' ((:) 'h' ((:) 's' ((:)
-                                        ' ' ((:) 't' ((:) 'r' ((:) 'a' ((:) 'f' ((:)
-                                        'f' ((:) 'i' ((:) 'c' ([]))))))))))))))
-                                      (hashWith (cipherHash c) ((:) (snd r) ((:) r0
-                                        []))) (hashDigestSize (cipherHash c))))))))))))))))))
+                                            (hkdfExpandLabel (cipherHash c)
+                                              (hkdfExtract (cipherHash c)
+                                                (b_replicate
+                                                  (hashDigestSize (cipherHash c))
+                                                  w0)
+                                                (b_replicate
+                                                  (hashDigestSize (cipherHash c))
+                                                  w0))
+                                              (s2b ((:) 'd' ((:) 'e' ((:) 'r' ((:)
+                                                'i' ((:) 'v' ((:) 'e' ((:) 'd'
+                                                ([])))))))))
+                                              (hashWith (cipherHash c) ((:)
+                                                (s2b ([])) []))
+                                              (hashDigestSize (cipherHash c)))
+                                            (ba_convert (snd p)))
+                                          (s2b ((:) 's' ((:) ' ' ((:) 'h' ((:) 's'
+                                            ((:) ' ' ((:) 't' ((:) 'r' ((:) 'a' ((:)
+                                            'f' ((:) 'f' ((:) 'i' ((:) 'c'
+                                            ([]))))))))))))))
+                                          (hashWith (cipherHash c) ((:) (snd r) ((:)
+                                            r0 [])))
+                                          (hashDigestSize (cipherHash c))))
+                                        ((Prelude.+) 1 ((Prelude.+) 1 0)))))))))))))))))))
                     (sum_merge
                       (prod_curry
                         (prod_curry
@@ -696,15 +852,15 @@ doHandshake_step =
                             (prod_curry
                               (prod_curry
                                 (prod_curry
-                                  (prod_curry (\_ r c p r0 r1 r2 r3 ->
-                                    lift_tls SendPacket (\r4 -> Prelude.Left ((,)
+                                  (prod_curry (\_ r c p r0 r1 r2 _ ->
+                                    lift_tls SendPacket (\r3 -> Prelude.Left ((,)
                                       (Prelude.Right (Prelude.Right (Prelude.Right
                                       (Prelude.Right (Prelude.Right (Prelude.Right
                                       (Prelude.Right (Prelude.Right (Prelude.Right
                                       (Prelude.Right (Prelude.Left ((,) ((,) ((,)
-                                      ((,) ((,) ((,) ((,) ((,) () r) c) p) r0) r1)
-                                      r2) r3) (unsafeCoerce r4)))))))))))))
-                                      (GHC.Base.Just (ExistT SendPacket
+                                      ((,) ((,) ((,) ((,) () r) c) p) r0) r1) r2)
+                                      (unsafeCoerce r3))))))))))))) (GHC.Base.Just
+                                      (ExistT SendPacket
                                       (unsafeCoerce ((,)
                                         (handshake13 ((:)
                                           (finished13
@@ -734,9 +890,10 @@ doHandshake_step =
                                                   (snd r) ((:) r0 [])))
                                                 (hashDigestSize (cipherHash c)))
                                               (hashWith (cipherHash c) ((:) 
-                                                (snd r) ((:) r0 ((:) r1 ((:) r3 ((:)
-                                                (unsafeCoerce r4) [])))))))) []))
-                                        (GHC.Base.Just ((,) ((,) (cipherHash c) c)
+                                                (snd r) ((:) r0 ((:) r1 ((:) r2 ((:)
+                                                (unsafeCoerce r3) [])))))))) []))
+                                        (GHC.Base.Just ((,) ((,) ((,) (cipherHash c)
+                                        c)
                                         (hkdfExpandLabel (cipherHash c)
                                           (hkdfExtract (cipherHash c)
                                             (hkdfExpandLabel (cipherHash c)
@@ -760,7 +917,9 @@ doHandshake_step =
                                             ([]))))))))))))))
                                           (hashWith (cipherHash c) ((:) (snd r) ((:)
                                             r0 [])))
-                                          (hashDigestSize (cipherHash c)))))))))))))))))))
+                                          (hashDigestSize (cipherHash c))))
+                                        ((Prelude.+) 1 ((Prelude.+) 1 ((Prelude.+) 1
+                                        0)))))))))))))))))))
                       (sum_merge
                         (prod_curry
                           (prod_curry
@@ -768,20 +927,17 @@ doHandshake_step =
                               (prod_curry
                                 (prod_curry
                                   (prod_curry
-                                    (prod_curry
-                                      (prod_curry (\_ r c p r0 r1 r2 r3 r4 ->
-                                        lift_tls SendPacket (\r5 -> Prelude.Left
-                                          ((,) (Prelude.Right (Prelude.Right
-                                          (Prelude.Right (Prelude.Right
-                                          (Prelude.Right (Prelude.Right
-                                          (Prelude.Right (Prelude.Right
-                                          (Prelude.Right (Prelude.Right
-                                          (Prelude.Right (Prelude.Left ((,) ((,)
-                                          ((,) ((,) ((,) ((,) ((,) ((,) ((,) () r)
-                                          c) p) r0) r1) r2) r3) r4)
-                                          (unsafeCoerce r5))))))))))))))
-                                          (GHC.Base.Just (ExistT RecvCCS
-                                          (unsafeCoerce ()))))))))))))))
+                                    (prod_curry (\_ r c p r0 r1 r2 r3 ->
+                                      lift_tls SendPacket (\r4 -> Prelude.Left ((,)
+                                        (Prelude.Right (Prelude.Right (Prelude.Right
+                                        (Prelude.Right (Prelude.Right (Prelude.Right
+                                        (Prelude.Right (Prelude.Right (Prelude.Right
+                                        (Prelude.Right (Prelude.Right (Prelude.Left
+                                        ((,) ((,) ((,) ((,) ((,) ((,) ((,) ((,) ()
+                                        r) c) p) r0) r1) r2) r3)
+                                        (unsafeCoerce r4))))))))))))))
+                                        (GHC.Base.Just (ExistT RecvCCS
+                                        (unsafeCoerce ())))))))))))))
                         (sum_merge
                           (prod_curry
                             (prod_curry
@@ -790,47 +946,44 @@ doHandshake_step =
                                   (prod_curry
                                     (prod_curry
                                       (prod_curry
-                                        (prod_curry
-                                          (prod_curry (\_ r c p r0 r1 r2 r3 r4 r5 ->
-                                            lift_tls RecvCCS (\_ -> Prelude.Left
-                                              ((,) (Prelude.Right (Prelude.Right
-                                              (Prelude.Right (Prelude.Right
-                                              (Prelude.Right (Prelude.Right
-                                              (Prelude.Right (Prelude.Right
-                                              (Prelude.Right (Prelude.Right
-                                              (Prelude.Right (Prelude.Right
-                                              (Prelude.Left ((,) ((,) ((,) ((,) ((,)
-                                              ((,) ((,) ((,) ((,) () r) c) p) r0)
-                                              r1) r2) r3) r4) r5))))))))))))))
-                                              (GHC.Base.Just (ExistT RecvFinished
-                                              (unsafeCoerce (GHC.Base.Just ((,) ((,)
-                                                (cipherHash c) c)
-                                                (hkdfExpandLabel (cipherHash c)
-                                                  (hkdfExtract (cipherHash c)
-                                                    (hkdfExpandLabel (cipherHash c)
-                                                      (hkdfExtract (cipherHash c)
-                                                        (b_replicate
-                                                          (hashDigestSize
-                                                            (cipherHash c)) w0)
-                                                        (b_replicate
-                                                          (hashDigestSize
-                                                            (cipherHash c)) w0))
-                                                      (s2b ((:) 'd' ((:) 'e' ((:)
-                                                        'r' ((:) 'i' ((:) 'v' ((:)
-                                                        'e' ((:) 'd' ([])))))))))
-                                                      (hashWith (cipherHash c) ((:)
-                                                        (s2b ([])) []))
-                                                      (hashDigestSize
-                                                        (cipherHash c)))
-                                                    (ba_convert (snd p)))
-                                                  (s2b ((:) 'c' ((:) ' ' ((:) 'h'
-                                                    ((:) 's' ((:) ' ' ((:) 't' ((:)
-                                                    'r' ((:) 'a' ((:) 'f' ((:) 'f'
-                                                    ((:) 'i' ((:) 'c'
-                                                    ([]))))))))))))))
-                                                  (hashWith (cipherHash c) ((:)
-                                                    (snd r) ((:) r0 [])))
-                                                  (hashDigestSize (cipherHash c))))))))))))))))))))
+                                        (prod_curry (\_ r c p r0 r1 r2 r3 r4 ->
+                                          lift_tls RecvCCS (\_ -> Prelude.Left ((,)
+                                            (Prelude.Right (Prelude.Right
+                                            (Prelude.Right (Prelude.Right
+                                            (Prelude.Right (Prelude.Right
+                                            (Prelude.Right (Prelude.Right
+                                            (Prelude.Right (Prelude.Right
+                                            (Prelude.Right (Prelude.Right
+                                            (Prelude.Left ((,) ((,) ((,) ((,) ((,)
+                                            ((,) ((,) ((,) () r) c) p) r0) r1) r2)
+                                            r3) r4)))))))))))))) (GHC.Base.Just
+                                            (ExistT RecvFinished
+                                            (unsafeCoerce (GHC.Base.Just ((,) ((,)
+                                              (cipherHash c) c)
+                                              (hkdfExpandLabel (cipherHash c)
+                                                (hkdfExtract (cipherHash c)
+                                                  (hkdfExpandLabel (cipherHash c)
+                                                    (hkdfExtract (cipherHash c)
+                                                      (b_replicate
+                                                        (hashDigestSize
+                                                          (cipherHash c)) w0)
+                                                      (b_replicate
+                                                        (hashDigestSize
+                                                          (cipherHash c)) w0))
+                                                    (s2b ((:) 'd' ((:) 'e' ((:) 'r'
+                                                      ((:) 'i' ((:) 'v' ((:) 'e'
+                                                      ((:) 'd' ([])))))))))
+                                                    (hashWith (cipherHash c) ((:)
+                                                      (s2b ([])) []))
+                                                    (hashDigestSize (cipherHash c)))
+                                                  (ba_convert (snd p)))
+                                                (s2b ((:) 'c' ((:) ' ' ((:) 'h' ((:)
+                                                  's' ((:) ' ' ((:) 't' ((:) 'r'
+                                                  ((:) 'a' ((:) 'f' ((:) 'f' ((:)
+                                                  'i' ((:) 'c' ([]))))))))))))))
+                                                (hashWith (cipherHash c) ((:)
+                                                  (snd r) ((:) r0 [])))
+                                                (hashDigestSize (cipherHash c)))))))))))))))))))
                           (sum_merge
                             (prod_curry
                               (prod_curry
@@ -839,77 +992,151 @@ doHandshake_step =
                                     (prod_curry
                                       (prod_curry
                                         (prod_curry
-                                          (prod_curry
-                                            (prod_curry
-                                              (\_ r c p r0 r1 r2 r3 r4 r5 ->
-                                              lift_tls RecvFinished (\r6 ->
-                                                Prelude.Left ((,)
-                                                (case byteString_beq
-                                                        (unsafeCoerce r6)
-                                                        (makeVerifyData
+                                          (prod_curry (\_ r c p r0 r1 r2 r3 r4 ->
+                                            lift_tls RecvFinished (\r5 ->
+                                              Prelude.Left ((,)
+                                              (case byteString_beq (unsafeCoerce r5)
+                                                      (makeVerifyData (cipherHash c)
+                                                        (hkdfExpandLabel
                                                           (cipherHash c)
-                                                          (hkdfExpandLabel
+                                                          (hkdfExtract
                                                             (cipherHash c)
-                                                            (hkdfExtract
+                                                            (hkdfExpandLabel
                                                               (cipherHash c)
-                                                              (hkdfExpandLabel
+                                                              (hkdfExtract
                                                                 (cipherHash c)
-                                                                (hkdfExtract
-                                                                  (cipherHash c)
-                                                                  (b_replicate
-                                                                    (hashDigestSize
-                                                                      (cipherHash c))
-                                                                    w0)
-                                                                  (b_replicate
-                                                                    (hashDigestSize
-                                                                      (cipherHash c))
-                                                                    w0))
-                                                                (s2b ((:) 'd' ((:)
-                                                                  'e' ((:) 'r' ((:)
-                                                                  'i' ((:) 'v' ((:)
-                                                                  'e' ((:) 'd'
-                                                                  ([])))))))))
-                                                                (hashWith
-                                                                  (cipherHash c)
-                                                                  ((:) (s2b ([]))
-                                                                  []))
-                                                                (hashDigestSize
-                                                                  (cipherHash c)))
-                                                              (ba_convert (snd p)))
-                                                            (s2b ((:) 'c' ((:) ' '
-                                                              ((:) 'h' ((:) 's' ((:)
-                                                              ' ' ((:) 't' ((:) 'r'
-                                                              ((:) 'a' ((:) 'f' ((:)
-                                                              'f' ((:) 'i' ((:) 'c'
-                                                              ([]))))))))))))))
-                                                            (hashWith (cipherHash c)
-                                                              ((:) (snd r) ((:) r0
-                                                              [])))
-                                                            (hashDigestSize
-                                                              (cipherHash c)))
+                                                                (b_replicate
+                                                                  (hashDigestSize
+                                                                    (cipherHash c))
+                                                                  w0)
+                                                                (b_replicate
+                                                                  (hashDigestSize
+                                                                    (cipherHash c))
+                                                                  w0))
+                                                              (s2b ((:) 'd' ((:) 'e'
+                                                                ((:) 'r' ((:) 'i'
+                                                                ((:) 'v' ((:) 'e'
+                                                                ((:) 'd'
+                                                                ([])))))))))
+                                                              (hashWith
+                                                                (cipherHash c) ((:)
+                                                                (s2b ([])) []))
+                                                              (hashDigestSize
+                                                                (cipherHash c)))
+                                                            (ba_convert (snd p)))
+                                                          (s2b ((:) 'c' ((:) ' '
+                                                            ((:) 'h' ((:) 's' ((:)
+                                                            ' ' ((:) 't' ((:) 'r'
+                                                            ((:) 'a' ((:) 'f' ((:)
+                                                            'f' ((:) 'i' ((:) 'c'
+                                                            ([]))))))))))))))
                                                           (hashWith (cipherHash c)
                                                             ((:) (snd r) ((:) r0
-                                                            ((:) r1 ((:) r3 ((:) r4
-                                                            ((:) r5 [])))))))) of {
-                                                  GHC.Base.True -> Prelude.Right
-                                                   (Prelude.Right (Prelude.Right
-                                                   (Prelude.Right (Prelude.Right
-                                                   (Prelude.Right (Prelude.Right
-                                                   (Prelude.Right (Prelude.Right
-                                                   (Prelude.Right (Prelude.Right
-                                                   (Prelude.Right (Prelude.Right
-                                                   (GHC.Base.Just ((,) ((,) ((,)
+                                                            [])))
+                                                          (hashDigestSize
+                                                            (cipherHash c)))
+                                                        (hashWith (cipherHash c)
+                                                          ((:) (snd r) ((:) r0 ((:)
+                                                          r1 ((:) r2 ((:) r3 ((:) r4
+                                                          [])))))))) of {
+                                                GHC.Base.True -> Prelude.Right
+                                                 (Prelude.Right (Prelude.Right
+                                                 (Prelude.Right (Prelude.Right
+                                                 (Prelude.Right (Prelude.Right
+                                                 (Prelude.Right (Prelude.Right
+                                                 (Prelude.Right (Prelude.Right
+                                                 (Prelude.Right (Prelude.Right
+                                                 (Prelude.Left ((,) ((,) ((,) ((,)
+                                                 ((,) ((,) ((,) ((,) () r) c) p) r0)
+                                                 r1) r2) r3) r4))))))))))))));
+                                                GHC.Base.False -> Prelude.Right
+                                                 (Prelude.Right (Prelude.Right
+                                                 (Prelude.Right (Prelude.Right
+                                                 (Prelude.Right (Prelude.Right
+                                                 (Prelude.Right (Prelude.Right
+                                                 (Prelude.Right (Prelude.Right
+                                                 (Prelude.Right (Prelude.Right
+                                                 (Prelude.Right
+                                                 GHC.Base.Nothing)))))))))))))})
+                                              (case byteString_beq (unsafeCoerce r5)
+                                                      (makeVerifyData (cipherHash c)
+                                                        (hkdfExpandLabel
+                                                          (cipherHash c)
+                                                          (hkdfExtract
+                                                            (cipherHash c)
+                                                            (hkdfExpandLabel
+                                                              (cipherHash c)
+                                                              (hkdfExtract
+                                                                (cipherHash c)
+                                                                (b_replicate
+                                                                  (hashDigestSize
+                                                                    (cipherHash c))
+                                                                  w0)
+                                                                (b_replicate
+                                                                  (hashDigestSize
+                                                                    (cipherHash c))
+                                                                  w0))
+                                                              (s2b ((:) 'd' ((:) 'e'
+                                                                ((:) 'r' ((:) 'i'
+                                                                ((:) 'v' ((:) 'e'
+                                                                ((:) 'd'
+                                                                ([])))))))))
+                                                              (hashWith
+                                                                (cipherHash c) ((:)
+                                                                (s2b ([])) []))
+                                                              (hashDigestSize
+                                                                (cipherHash c)))
+                                                            (ba_convert (snd p)))
+                                                          (s2b ((:) 'c' ((:) ' '
+                                                            ((:) 'h' ((:) 's' ((:)
+                                                            ' ' ((:) 't' ((:) 'r'
+                                                            ((:) 'a' ((:) 'f' ((:)
+                                                            'f' ((:) 'i' ((:) 'c'
+                                                            ([]))))))))))))))
+                                                          (hashWith (cipherHash c)
+                                                            ((:) (snd r) ((:) r0
+                                                            [])))
+                                                          (hashDigestSize
+                                                            (cipherHash c)))
+                                                        (hashWith (cipherHash c)
+                                                          ((:) (snd r) ((:) r0 ((:)
+                                                          r1 ((:) r2 ((:) r3 ((:) r4
+                                                          [])))))))) of {
+                                                GHC.Base.True -> GHC.Base.Just
+                                                 (ExistT SendPacket
+                                                 (unsafeCoerce ((,)
+                                                   (appData13
+                                                     (s2b ((:) 'h' ((:) 'e' ((:) 'l'
+                                                       ((:) 'l' ((:) 'o' ((:) ' '
+                                                       ([]))))))))) (GHC.Base.Just
+                                                   ((,) ((,) ((,) (cipherHash c) c)
                                                    (hkdfExpandLabel (cipherHash c)
                                                      (hkdfExtract (cipherHash c)
                                                        (hkdfExpandLabel
                                                          (cipherHash c)
                                                          (hkdfExtract (cipherHash c)
-                                                           (b_replicate
+                                                           (hkdfExpandLabel
+                                                             (cipherHash c)
+                                                             (hkdfExtract
+                                                               (cipherHash c)
+                                                               (b_replicate
+                                                                 (hashDigestSize
+                                                                   (cipherHash c))
+                                                                 w0)
+                                                               (b_replicate
+                                                                 (hashDigestSize
+                                                                   (cipherHash c))
+                                                                 w0))
+                                                             (s2b ((:) 'd' ((:) 'e'
+                                                               ((:) 'r' ((:) 'i'
+                                                               ((:) 'v' ((:) 'e'
+                                                               ((:) 'd' ([])))))))))
+                                                             (hashWith
+                                                               (cipherHash c) ((:)
+                                                               (s2b ([])) []))
                                                              (hashDigestSize
-                                                               (cipherHash c)) w0)
-                                                           (b_replicate
-                                                             (hashDigestSize
-                                                               (cipherHash c)) w0))
+                                                               (cipherHash c)))
+                                                           (ba_convert (snd p)))
                                                          (s2b ((:) 'd' ((:) 'e' ((:)
                                                            'r' ((:) 'i' ((:) 'v'
                                                            ((:) 'e' ((:) 'd'
@@ -918,31 +1145,38 @@ doHandshake_step =
                                                            ((:) (s2b ([])) []))
                                                          (hashDigestSize
                                                            (cipherHash c)))
-                                                       (ba_convert (snd p)))
-                                                     (s2b ((:) 's' ((:) ' ' ((:) 'h'
-                                                       ((:) 's' ((:) ' ' ((:) 't'
+                                                       (b_replicate
+                                                         (hashDigestSize
+                                                           (cipherHash c)) w0))
+                                                     (s2b ((:) 's' ((:) ' ' ((:) 'a'
+                                                       ((:) 'p' ((:) ' ' ((:) 't'
                                                        ((:) 'r' ((:) 'a' ((:) 'f'
                                                        ((:) 'f' ((:) 'i' ((:) 'c'
                                                        ([]))))))))))))))
                                                      (hashWith (cipherHash c) ((:)
-                                                       (snd r) ((:) r0 [])))
-                                                     (hashDigestSize (cipherHash c)))
-                                                   (hashWith (cipherHash c) ((:)
-                                                     (snd r) ((:) r0 ((:) r1 ((:) r3
-                                                     ((:) r4 [])))))))
-                                                   (makeCertVerify (snd r2)
-                                                     (hashWith (cipherHash c) ((:)
                                                        (snd r) ((:) r0 ((:) r1 ((:)
-                                                       r3 [])))))))
-                                                   (fst r2)))))))))))))));
-                                                  GHC.Base.False -> Prelude.Right
-                                                   (Prelude.Right (Prelude.Right
-                                                   (Prelude.Right (Prelude.Right
-                                                   (Prelude.Right (Prelude.Right
-                                                   (Prelude.Right (Prelude.Right
-                                                   (Prelude.Right (Prelude.Right
-                                                   (Prelude.Right (Prelude.Right
-                                                   GHC.Base.Nothing))))))))))))})
-                                                GHC.Base.Nothing))))))))))))
-                            (\o _ _ -> Prelude.Right o)))))))))))))
+                                                       r2 ((:) r3 ((:) r4 [])))))))
+                                                     (hashDigestSize (cipherHash c))))
+                                                   0)))));
+                                                GHC.Base.False -> GHC.Base.Nothing}))))))))))))
+                            (sum_merge
+                              (prod_curry
+                                (prod_curry
+                                  (prod_curry
+                                    (prod_curry
+                                      (prod_curry
+                                        (prod_curry
+                                          (prod_curry
+                                            (prod_curry (\_ _ _ _ _ _ _ _ _ ->
+                                              lift_tls SendPacket (\_ ->
+                                                Prelude.Left ((,) (Prelude.Right
+                                                (Prelude.Right (Prelude.Right
+                                                (Prelude.Right (Prelude.Right
+                                                (Prelude.Right (Prelude.Right
+                                                (Prelude.Right (Prelude.Right
+                                                (Prelude.Right (Prelude.Right
+                                                (Prelude.Right (Prelude.Right
+                                                (Prelude.Right (GHC.Base.Just
+                                                ()))))))))))))))) GHC.Base.Nothing)))))))))))
+                              (\o _ _ -> Prelude.Right o))))))))))))))
 
